src/gsim/gSimMemory.v
@@ -34,14 +34,18 @@ Set Implicit Arguments.
 
 Definition world: Type. Admitted.
 Definition world_le: world -> world -> Prop. Admitted.
-Definition world_le_PreOrder: PreOrder world_le. Admitted.
+Instance world_le_PreOrder: PreOrder world_le. Admitted.
 
 Definition sim_memory: forall (w: world) (mem_src mem_tgt:Memory.t), Prop. Admitted.
 Definition sim_timemap: forall (w: world) (sc_src sc_tgt: TimeMap.t), Prop. Admitted.
 Definition sim_local: forall (w: world) (lc_src lc_tgt:Local.t), Prop. Admitted.
 
-Lemma sim_local_world_mon: forall (w0 w1: world) (WORLD: world_le w0 w1),
+Definition sim_local_world_mon: forall (w0 w1: world) (WORLD: world_le w0 w1),
     sim_local w0 <2= sim_local w1.
+Admitted.
+
+Definition sim_timemap_world_mon: forall (w0 w1: world) (WORLD: world_le w0 w1),
+    sim_timemap w0 <2= sim_timemap w1.
 Admitted.
 
 Lemma sim_local_memory_bot:
@@ -68,4 +72,24 @@ Lemma sim_memory_cap: forall
       (<<TIMEMAP: sim_timemap w2 sc1_src sc1_tgt>>) /\
       (<<WORLD: world_le w1 w2>>)
 .
+Admitted.
+
+Lemma sim_local_promise
+      w0
+      lc1_src mem1_src
+      lc1_tgt mem1_tgt
+      lc2_tgt mem2_tgt
+      loc from to msg_tgt kind_tgt
+      (STEP_TGT: Local.promise_step lc1_tgt mem1_tgt loc from to msg_tgt lc2_tgt mem2_tgt kind_tgt)
+      (LOCAL1: sim_local w0 lc1_src lc1_tgt)
+      (MEM1: sim_memory w0 mem1_src mem1_tgt)
+      (WF1_SRC: Local.wf lc1_src mem1_src)
+      (WF1_TGT: Local.wf lc1_tgt mem1_tgt)
+      (MEM1_SRC: Memory.closed mem1_src)
+      (MEM1_TGT: Memory.closed mem1_tgt):
+  exists lc2_src mem2_src msg_src kind_src w1,
+    (<<STEP_SRC: Local.promise_step lc1_src mem1_src loc from to msg_src lc2_src mem2_src kind_src>>) /\
+    (<<LOCAL2: sim_local w1 lc2_src lc2_tgt>>) /\
+    (<<MEM2: sim_memory w1 mem2_src mem2_tgt>>) /\
+    (<<WORLD: world_le w0 w1>>).
 Admitted.
